\chapter{De afledte af $\sqrt{1-x^2}$}
\label{app:afledte}
De afledte til $g(x)$, differentieret med k√¶dereglen og produktreglen;
\begin{align*}
g(x) &= \sqrt{1-x^2} \\
\end{align*}
\begin{align*}
g'(x) &= \frac{1}{2\sqrt{1-x^2}} (-2x)\\
&= \frac{-x}{\sqrt{1-x^2}} \\
\end{align*}
\begin{align*}
g''(x) &= \frac{-1}{\sqrt{1-x^2}} -x\left(\frac{-1}{2}\right)(-2x)\frac{1}{\sqrt{1-x^2}(1-x^2)}\\
&= \frac{-1}{\sqrt{1-x^2}} -\frac{x^2}{\sqrt{1-x^2}(1-x^2)}\\
&= \frac{-1}{\sqrt{1-x^2}}\left(\frac{x^2}{1-x^2}+1\right)\\
\end{align*}
\begin{align*}
g^{(3)}(x) &= \frac{-x}{\sqrt{1-x^2}(1-x^2)}\left(\frac{x^2}{1-x^2}+1\right)- \frac{1}{\sqrt{1-x^2}}\left(\frac{2x}{1-x^2}+\frac{2x^3}{(1-x^2)^2}\right)\\
&= \frac{-1}{\sqrt{1-x^2}}\left(\frac{x^3}{(1-x^2)^2}+\frac{x}{1-x^2}\right)- \frac{1}{\sqrt{1-x^2}}\left(\frac{2x}{1-x^2}+\frac{2x^3}{(1-x^2)^2}\right)\\
&=\frac{-1}{\sqrt{1-x^2}}\left(\frac{3x^3}{(1-x^2)^2}+\frac{3x}{1-x^2}\right) \\
\end{align*}
\begin{align*}
g^{(4)}(x) &= \frac{-x}{\sqrt{1-x^2}(1-x^2)}\left(\frac{3x^3}{(1-x^2)^2}+\frac{3x}{1-x^2}\right)-\frac{1}{\sqrt{1-x^2}}\left(\frac{9x^2}{(1-x^2)^2}+\frac{12x^4}{(1-x^2)^3}+\frac{3}{1-x^2}+\frac{6x^2}{(1-x^2)^2}\right) \\
&= \frac{-1}{\sqrt{1-x^2}}\left(\frac{3x^4}{(1-x^2)^3}+\frac{3x^2}{(1-x^2)^2}\right)-\frac{1}{\sqrt{1-x^2}}\left(\frac{9x^2}{(1-x^2)^2}+\frac{12x^4}{(1-x^2)^3}+\frac{3}{1-x^2}+\frac{6x^2}{(1-x^2)^2}\right) \\
&= \frac{-1}{\sqrt{1-x^2}} \left(\frac{15x^4}{(1-x^2)^3}+\frac{18x^2}{(1-x^2)^2}+\frac{3}{1-x^2}\right)\\
\end{align*}